TransVal/transval.v
@@ -1,0 +1,13 @@
+Require Import List.
+Require Import IL Exp Coherence sexp smt.
+
+Lemma models_if_eval :
+forall s D E s' E', 
+ssa  s D
+-> ((nil, E,s) -> (nil, E',s'))
+-> forall p, models E'  (translateStmt s p).
+(*
+*** Local Variables: ***
+*** coq-load-path: (("../" "Lvc")) ***
+*** End: ***
+*)
